trying to make sense of class elaboration

Translation/Global.lean
@@ -9,37 +9,56 @@ import Translation.Term
 
 
 
-inductive Translation.GlobalWf : Surface.GlobalEnv -> Core.GlobalEnv -> Surface.Global -> Prop where
-| data {ctors : Vect n (String × Surface.Ty)} {G : Surface.GlobalEnv}{G' : Core.GlobalEnv}:
-  (∀ i y T, ctors i = (y, T) ->
-    (Surface.Global.data x K Vect.nil :: G)&[] ⊢s T : `★
-    ∧ Surface.ValidCtor x T
-    ∧ x ≠ y
-    ∧ Surface.lookup y G = none) ->
-  (∀ i j, (ctors i).1 ≠ (ctors j).1) ->
+-- inductive Translation.GlobalWf : Surface.GlobalEnv -> Core.GlobalEnv -> Surface.Global -> Prop where
+-- | data {ctors : Vect n (String × Surface.Ty)} {G : Surface.GlobalEnv}{G' : Core.GlobalEnv}:
+--   (∀ i y T, ctors i = (y, T) ->
+--     (Surface.Global.data x K Vect.nil :: G)&[] ⊢s T : `★
+--     ∧ Surface.ValidCtor x T
+--     ∧ x ≠ y
+--     ∧ Surface.lookup y G = none) ->
+--   (∀ i j, (ctors i).1 ≠ (ctors j).1) ->
+--   Surface.lookup x G = none ->
+--   GlobalWf G G' (Surface.Global.data x K ctors)
+-- | defn :
+--   Surface.lookup x G = none ->
+--   G&[] ⊢s T : `★ ->
+--   Surface.Term.Elab G G' .chk [] [] t T t' ->
+--   GlobalWf G G' (Surface.Global.defn x T t)
+-- | classDecl :
+--   Surface.lookup s G = none ->
+--   Surface.ValidOpenKind K ->
+--   (∀ i j, (ms i).1 ≠ (ms j).1) ->
+--   (∀ i y T, ms i = (y, T) ->
+--     (Surface.Global.classDecl s K Vect.nil :: G)&[] ⊢s T : `★
+--     ∧ Surface.ValidClassMethodTy s T
+--     ∧ s ≠ y
+--     ∧ Surface.lookup y G = none) ->
+--   GlobalWf G G' (Surface.Global.classDecl s K ms)
+-- | instDecl :
+--   Surface.ValidClassInstTy C T ->
+--   -- TODO: Do Non-overlapping check here
+--   Surface.lookup C G = some (.opent C K ms') ->
+--   -- TODO: check for method types
+--   GlobalWf G G' (.instDecl T ms)
+
+
+inductive ValidClassDecl (G : Surface.GlobalEnv) (G' : Core.GlobalEnv) (x : String) (K: Surface.Kind) :
+          {n : Nat} -> (Vect n (String × Surface.Ty)) -> Core.GlobalEnv -> Prop where
+| nil :
   Surface.lookup x G = none ->
-  GlobalWf G G' (Surface.Global.data x K ctors)
-| defn :
-  Surface.lookup x G = none ->
-  G&[] ⊢s T : `★ ->
-  Surface.Term.Elab G G' .chk [] [] t T t' ->
-  GlobalWf G G' (Surface.Global.defn x T t)
-| classDecl :
-  Surface.lookup s G = none ->
   Surface.ValidOpenKind K ->
-  (∀ i j, (ms i).1 ≠ (ms j).1) ->
-  (∀ i y T, ms i = (y, T) ->
-    (Surface.Global.classDecl s K Vect.nil :: G)&[] ⊢s T : `★
-    ∧ Surface.ValidClassMethodTy s T
-    ∧ s ≠ y
-    ∧ Surface.lookup y G = none) ->
-  GlobalWf G G' (Surface.Global.classDecl s K ms)
-| instDecl :
-  Surface.ValidClassInstTy C T ->
-  -- TODO: Do Non-overlapping check here
-  Surface.lookup C G = some (.opent C K ms') ->
-  -- TODO: check for method types
-  GlobalWf G G' (.instDecl T ms)
+  ValidClassDecl G G' x K Vect.nil (List.cons (.opent x K.translate) G')
+| cons {n : Nat} {ms : Vect n (String × Surface.Ty)} :
+  ms' = ms.to_list.map (λ (x, τ) => Core.Global.openm x τ.translate) ->
+  ValidClassDecl G G' x K ms (ms' ++ List.cons (.opent x K.translate) G')  ->
+
+  -- method names are unique
+  Surface.lookup m (.classDecl x K ms :: G) = none ->
+
+  -- method type is okay
+  Surface.ValidClassMethodTy x τ ->
+
+  ValidClassDecl G G' x K (n := n + 1) (Vect.cons (m , τ) ms) (List.cons (Core.Global.openm m τ.translate) (ms' ++ List.cons (.opent x K.translate) G'))
 
 
 
@@ -70,20 +89,21 @@ inductive Surface.Global.Elab : Surface.GlobalEnv -> Core.GlobalEnv -> Prop
 
   Surface.Global.Elab (.cons (.data (n := n) x K ctors) G) (.cons (.data n x K.translate ctors') G')
 
-| classDecl {n : Nat} {ms : Vect n (String × Ty)} {ms' : Vect n Core.Global} :
+| classDecl {n : Nat} {ms : Vect n (String × Ty)} {ms' : Core.GlobalEnv} :
   Surface.Global.Elab G G' ->
 
-  Surface.lookup x G = none ->
-  Surface.ValidOpenKind K ->
-  (∀ i j, (ms i).1 ≠ (ms j).1) ->
-  (∀ i y T, ms i = (y, T) ->
-    (Surface.Global.classDecl x K Vect.nil :: G)&[] ⊢s T : `★
-    ∧ Surface.ValidClassMethodTy x T
-    ∧ x ≠ y
-    ∧ Surface.lookup y G = none) ->
-  ms' = (λ i => Core.Global.openm (ms i).1 (ms i).2.translate) ->
+  ValidClassDecl G G' x K ms ms' ->
+  -- (∀ i j, (ms i).1 ≠ (ms j).1) ->
+  -- (∀ i y T, ms i = (y, T) ->
+  --   (Surface.Global.classDecl x K Vect.nil :: G)&[] ⊢s T : `★
+  --   ∧ Surface.ValidClassMethodTy x T
+  --   ∧ x ≠ y
+  --   ∧ Surface.lookup y G = none) ->
+  -- ms' = ms.to_list.foldr (λ (mth : String × Ty) acc =>
+  --       List.cons (Core.Global.openm mth.1 mth.2.translate) acc)
+  --       (List.cons (Core.Global.opent x K.translate) G') ->
 
-  Surface.Global.Elab ((.classDecl x K ms) :: G) (ms'.to_list ++ (Core.Global.opent x K.translate :: G'))
+  Surface.Global.Elab ((.classDecl x K ms) :: G) ms'
 
 
 notation:170 G:170 " -↪ " G':170 => Surface.Global.Elab G G'
